Axioms_Quantum.thy
@@ -1,12 +1,16 @@
 (* AXIOM INSTANTIATION (use instantiate_laws.py to generate Laws_Quantum.thy)
 
+    # Type classe
     domain \<rightarrow> finite
+    
+    # Constants
     comp_update \<rightarrow> timesOp
     id_update \<rightarrow> idOp
     update_hom \<rightarrow> clinear
     update_2hom \<rightarrow> cbilinear
     tensor_update \<rightarrow> tensor_op
     
+    # Lemmas
     id_update_left \<rightarrow> times_idOp2
     id_update_right \<rightarrow> times_idOp1
     comp_update_assoc \<rightarrow> cblinfun_apply_assoc
@@ -28,46 +32,15 @@ begin
 unbundle cblinfun_notation
 no_notation m_inv ("inv\<index> _" [81] 80)
 
-
 type_synonym 'a update = \<open>('a ell2, 'a ell2) cblinfun\<close>
-
-(* abbreviation (input) comp_update :: "'a update \<Rightarrow> 'a update \<Rightarrow> 'a update" where
-  "comp_update \<equiv> timesOp" *)
-
-(* abbreviation id_update :: "'a update" where
-  "id_update \<equiv> idOp" *)
-
-(* lemma id_update_left: "timesOp idOp a = a"
-  by simp *)
-(* lemma id_update_right: "timesOp a idOp = a"
-  by simp *)
-
-(* lemma comp_update_assoc: "timesOp (timesOp a b) c = timesOp a (timesOp b c)"
-  by (simp add: cblinfun_apply_assoc) *)
-
-
-type_synonym ('a,'b) update_hom = \<open>'a update \<Rightarrow> 'b update\<close>
-(* abbreviation (input) update_hom :: \<open>('a,'b) update_hom \<Rightarrow> bool\<close> where
-  "update_hom \<equiv> clinear" *)
-
-(* lemma id_update_hom: \<open>clinear id\<close>
-  by (fact complex_vector.linear_id) *)
-
-(* lemma comp_update_hom: "clinear F \<Longrightarrow> clinear G \<Longrightarrow> clinear (G \<circ> F)"
-  by (simp add: Complex_Vector_Spaces.linear_compose)  *)
-
-type_synonym ('a,'b,'c) update_2hom = \<open>'a update \<Rightarrow> 'b update \<Rightarrow> 'c update\<close>
-(* abbreviation (input) update_2hom :: "('a, 'b, 'c) update_2hom \<Rightarrow> bool" where
-  "update_2hom \<equiv> cbilinear" *)
-
-(* lemma update_2hom_bilinear: "update_2hom F \<longleftrightarrow> cbilinear F"
-  by (meson cbilinear_def update_2hom_def update_hom_def) *)
+(* type_synonym ('a,'b) update_hom = \<open>'a update \<Rightarrow> 'b update\<close> *)
+(* type_synonym ('a,'b,'c) update_2hom = \<open>'a update \<Rightarrow> 'b update \<Rightarrow> 'c update\<close> *)
 
 lemma update_hom_o_2hom_is_2hom: \<open>cbilinear F2 \<Longrightarrow> clinear G \<Longrightarrow> cbilinear (\<lambda>a b. G (F2 a b))\<close>
   apply (auto simp: cbilinear_def intro!: clinearI)
   apply (smt (z3) clinear_additive_D)
   apply (metis complex_vector.linear_scale)
-  apply (simp add: clinear_additive_D)
+   apply (simp add: clinear_additive_D)
   by (simp add: complex_vector.linear_scale)
 lemma update_2hom_o_hom_left_is_hom: \<open>cbilinear F2 \<Longrightarrow> clinear G \<Longrightarrow> cbilinear (\<lambda>a b. F2 (G a) b)\<close>
   apply (auto simp: cbilinear_def intro!: clinearI)
@@ -78,34 +51,7 @@ lemma update_2hom_sym: \<open>cbilinear F2 \<Longrightarrow> cbilinear (\<lambda
 lemma update_2hom_left_is_hom: \<open>cbilinear F2 \<Longrightarrow> clinear (\<lambda>a. F2 a b)\<close>
   by (auto simp: cbilinear_def)
 
-
-(* lemma comp_update_is_2hom: "cbilinear timesOp"
-  by (auto intro!: clinearI simp add: cbilinear_def cblinfun_apply_dist1 cblinfun_apply_dist2) *)
-
-(* abbreviation tensor_update :: \<open>'a::finite update \<Rightarrow> 'b::finite update \<Rightarrow> ('a\<times>'b) update\<close> where
-  \<open>tensor_update \<equiv> tensor_op\<close> *)
-                 
-(* lemma tensor_update_mult: \<open>timesOp (tensor_op a c) (tensor_op b d) = tensor_op (timesOp a b) (timesOp c d)\<close>
-  for a :: "_::finite ell2 \<Rightarrow>\<^sub>C\<^sub>L _::finite ell2" and b :: "_::finite ell2 \<Rightarrow>\<^sub>C\<^sub>L _::finite ell2" and
-  c :: "_::finite ell2 \<Rightarrow>\<^sub>C\<^sub>L _ ell2" and d :: "_::finite ell2 \<Rightarrow>\<^sub>C\<^sub>L _ ell2"
-  by (rule comp_tensor_op) *)
-
-(* lemmas tensor_update_is_2hom = tensor_op_cbilinear *)
-
-(* definition assoc :: \<open>(('a::finite\<times>'b::finite)\<times>'c::finite, 'a\<times>('b\<times>'c)) clinear\<close> where
-  \<open>assoc a = assoc_ell2 o\<^sub>C\<^sub>L a o\<^sub>C\<^sub>L assoc_ell2'\<close>
-
-lemma assoc_is_hom: \<open>clinear assoc\<close>
-  unfolding assoc_def
-  by (simp add: cblinfun_apply_dist1 cblinfun_apply_dist2 clinearI)
-
-lemma assoc_apply: \<open>assoc (tensor_op (tensor_op a b) c) = tensor_op a (tensor_op b c)\<close>
-  apply (rule equal_ket)
-  apply (case_tac x)
-  by (simp add: assoc_def times_applyOp tensor_op_ell2 assoc_ell2_tensor assoc_ell2'_tensor flip: tensor_ell2_ket) *)
-
-
-definition lvalue :: \<open>('a, 'b) update_hom \<Rightarrow> bool\<close> where
+definition lvalue :: \<open>('a::finite update \<Rightarrow> 'b::finite update) \<Rightarrow> bool\<close> where
   "lvalue F \<longleftrightarrow> 
      clinear F
    \<and> F idOp = idOp 
@@ -116,17 +62,14 @@ lemma lvalue_of_id: \<open>lvalue F \<Longrightarrow> F idOp = idOp\<close>
   by (simp add: lvalue_def)
 
 lemma lvalue_hom: "lvalue F \<Longrightarrow> clinear F"
-  for F :: "('a,'b) update_hom" and G :: "('b,'c) update_hom"
   unfolding lvalue_def by simp
 
 lemma lvalue_comp: "lvalue F \<Longrightarrow> lvalue G \<Longrightarrow> lvalue (G \<circ> F)"
-  for F :: "('a,'b) update_hom" and G :: "('b,'c) update_hom" 
   unfolding lvalue_def
   apply auto
   using Complex_Vector_Spaces.linear_compose by blast
 
 lemma lvalue_mult: "lvalue F \<Longrightarrow> timesOp (F a) (F b) = F (timesOp a b)"
-  for F :: "('a,'b) update_hom" and G :: "('b,'c) update_hom" 
   unfolding lvalue_def
   by auto
 
@@ -137,15 +80,14 @@ lemma lvalue_tensor_right: \<open>lvalue (\<lambda>a. tensor_op idOp a)\<close>
   apply (simp add: comp_tensor_op lvalue_def tensor_op_cbilinear tensor_op_adjoint)
   by (meson cbilinear_def tensor_op_cbilinear)
 
-
 lemma pair_lvalue_axiom: 
-  fixes F :: \<open>('a::finite, 'c) update_hom\<close> and G :: \<open>('b::finite, 'c) update_hom\<close>
+  fixes F :: \<open>'a::finite update \<Rightarrow> 'c::finite update\<close> and G :: \<open>'b::finite update \<Rightarrow> 'c update\<close>
   assumes \<open>lvalue F\<close> and \<open>lvalue G\<close> and [simp]: \<open>clinear p\<close>
   assumes compat: \<open>\<And>a b. F a o\<^sub>C\<^sub>L G b = G b o\<^sub>C\<^sub>L F a\<close>
   assumes tensor: \<open>\<And>a b. p (tensor_op a b) = F a o\<^sub>C\<^sub>L G b\<close>
   shows \<open>lvalue p\<close>
 proof (unfold lvalue_def, intro conjI allI)
-  have h1: \<open>clinear (\<lambda>a. p (a o\<^sub>C\<^sub>L b))\<close> for b
+  have h1: \<open>clinear (\<lambda>a. p (a o\<^sub>C\<^sub>L b))\<close> for b :: "('a \<times> 'b) update"
     apply (rule linear_compose[unfolded o_def, of _ p])
      apply (simp add: cblinfun_apply_dist1 clinearI)
     by simp
@@ -153,7 +95,7 @@ proof (unfold lvalue_def, intro conjI allI)
     apply (rule linear_compose[unfolded o_def, of p])
     apply simp
     by (meson cblinfun_apply_dist1 clinearI scalar_op_op)
-  have h3: \<open>clinear (\<lambda>c. p (d o\<^sub>C\<^sub>L c))\<close> for d
+  have h3: \<open>clinear (\<lambda>c. p (d o\<^sub>C\<^sub>L c))\<close> for d :: "('a \<times> 'b) update"
     apply (rule linear_compose[unfolded o_def, of _ p])
      apply (simp add: cblinfun_apply_dist2 clinearI)
     by simp
