QHoare.thy
@@ -8,22 +8,16 @@ locale qhoare =
   fixes memory_type :: "'mem::finite itself"
 begin
 
-definition "apply U R = R U" for R :: \<open>('a,'mem) update_hom\<close>
-definition "ifthen R x = R (butterket x x)" for R :: \<open>('a,'mem) update_hom\<close>
+definition "apply U R = R U" for R :: \<open>'a update \<Rightarrow> 'mem update\<close>
+definition "ifthen R x = R (butterket x x)" for R :: \<open>'a update \<Rightarrow> 'mem update\<close>
 definition "program S = fold (o\<^sub>C\<^sub>L) S idOp" for S :: \<open>'mem update list\<close>
 
 
 definition hoare :: \<open>'mem ell2 clinear_space \<Rightarrow> ('mem ell2 \<Rightarrow>\<^sub>C\<^sub>L 'mem ell2) list \<Rightarrow> 'mem ell2 clinear_space \<Rightarrow> bool\<close> where
   "hoare C p D \<longleftrightarrow> (\<forall>\<psi>\<in>space_as_set C. program p *\<^sub>V \<psi> \<in> space_as_set D)" for C p D
 
-(* abbreviation (input) "EQP R \<psi> \<equiv> R (selfbutter \<psi>)" for R :: \<open>('a,'mem) update_hom\<close> *)
-definition EQ :: "('a,'mem) update_hom \<Rightarrow> 'a ell2 \<Rightarrow> 'mem ell2 clinear_space" (infix "=\<^sub>q" 75) where
-  "EQ R \<psi> = R (selfbutter \<psi>) *\<^sub>S \<top>" for R :: \<open>('a,'mem) update_hom\<close>
-
-(* lemma swap_EQP':
-  assumes "compatible R S"
-  shows "EQP R \<psi> o\<^sub>C\<^sub>L (EQP S \<phi> o\<^sub>C\<^sub>L C) = EQP S \<phi> o\<^sub>C\<^sub>L (EQP R \<psi> o\<^sub>C\<^sub>L C)"
-  by (simp add: assoc_left(1) swap_lvalues[OF assms]) *)
+definition EQ :: "('a update \<Rightarrow> 'mem update) \<Rightarrow> 'a ell2 \<Rightarrow> 'mem ell2 clinear_space" (infix "=\<^sub>q" 75) where
+  "EQ R \<psi> = R (selfbutter \<psi>) *\<^sub>S \<top>"
 
 lemma join_EQP:
   assumes [compatible]: "compatible R S"
@@ -66,7 +60,7 @@ lemma hoare_apply:
   by (metis (no_types, lifting) applyOpSpace.rep_eq closure_subset imageI less_eq_clinear_space.rep_eq subsetD)
 
 lemma hoare_ifthen: 
-  fixes R :: \<open>('a,'mem) update_hom\<close>
+  fixes R :: \<open>'a update \<Rightarrow> 'mem update\<close>
   assumes "R (selfbutter (ket x)) *\<^sub>S pre \<le> post"
   shows "hoare pre [ifthen R x] post"
   using assms 
